<?xml version="1.0"?>
<rdf:RDF xmlns="http://ontology.foodlog.eu#"
     xml:base="http://ontology.foodlog.eu"
     xmlns:owl="http://www.w3.org/2002/07/owl#"
     xmlns:rdf="http://www.w3.org/1999/02/22-rdf-syntax-ns#"
     xmlns:xml="http://www.w3.org/XML/1998/namespace"
     xmlns:xsd="http://www.w3.org/2001/XMLSchema#"
     xmlns:obda="https://w3id.org/obda/vocabulary#"
     xmlns:rdfs="http://www.w3.org/2000/01/rdf-schema#"
     xmlns:swrl="http://www.w3.org/2003/11/swrl#"
     xmlns:swrlb="http://www.w3.org/2003/11/swrlb#"
     xmlns:recipes="http://ontology.foodlog.eu#">
    <owl:Ontology rdf:about="http://ontology.foodlog.eu"/>
    


    <!-- 
    ///////////////////////////////////////////////////////////////////////////////////////
    //
    // Object Properties
    //
    ///////////////////////////////////////////////////////////////////////////////////////
     -->

    


    <!-- http://ontology.foodlog.eu#amountOf -->

    <owl:ObjectProperty rdf:about="http://ontology.foodlog.eu#amountOf">
        <rdfs:domain rdf:resource="http://ontology.foodlog.eu#UsesIngredient"/>
        <rdfs:range rdf:resource="http://ontology.foodlog.eu#Ingredient"/>
        <rdfs:comment xml:lang="en">An amount of the ingredient is used</rdfs:comment>
        <rdfs:label>Amount of</rdfs:label>
    </owl:ObjectProperty>
    


    <!-- http://ontology.foodlog.eu#belongsTo -->

    <owl:ObjectProperty rdf:about="http://ontology.foodlog.eu#belongsTo">
        <rdfs:domain rdf:resource="http://ontology.foodlog.eu#Ingredient"/>
        <rdfs:range rdf:resource="http://ontology.foodlog.eu#FoodType"/>
        <rdfs:comment xml:lang="en">The ingredient belongs to a certain food type.</rdfs:comment>
        <rdfs:label>Belongs to</rdfs:label>
    </owl:ObjectProperty>
    


    <!-- http://ontology.foodlog.eu#hasNutritionFacts -->

    <owl:ObjectProperty rdf:about="http://ontology.foodlog.eu#hasNutritionFacts">
        <rdfs:domain rdf:resource="http://ontology.foodlog.eu#Ingredient"/>
        <rdfs:range rdf:resource="http://ontology.foodlog.eu#NutritionFacts"/>
        <rdfs:comment xml:lang="en">The quantity of nutrients that is present in 100 grams of a certain ingredient.</rdfs:comment>
        <rdfs:label>Has nutrition facts</rdfs:label>
    </owl:ObjectProperty>
    


    <!-- http://ontology.foodlog.eu#hasStep -->

    <owl:ObjectProperty rdf:about="http://ontology.foodlog.eu#hasStep">
        <rdfs:domain rdf:resource="http://ontology.foodlog.eu#RecipeVariant"/>
        <rdfs:range rdf:resource="http://ontology.foodlog.eu#RecipeStep"/>
        <rdfs:comment xml:lang="en">A recipe variant has a recipe step.</rdfs:comment>
        <rdfs:label xml:lang="en">Has step</rdfs:label>
    </owl:ObjectProperty>
    


    <!-- http://ontology.foodlog.eu#hasVariant -->

    <owl:ObjectProperty rdf:about="http://ontology.foodlog.eu#hasVariant">
        <rdfs:domain rdf:resource="http://ontology.foodlog.eu#Recipe"/>
        <rdfs:range rdf:resource="http://ontology.foodlog.eu#RecipeVariant"/>
        <rdfs:comment xml:lang="en">A recipe has a recipe variant.</rdfs:comment>
        <rdfs:label xml:lang="en">Has variant</rdfs:label>
    </owl:ObjectProperty>
    


    <!-- http://ontology.foodlog.eu#usesAmount -->

    <owl:ObjectProperty rdf:about="http://ontology.foodlog.eu#usesAmount">
        <rdfs:domain rdf:resource="http://ontology.foodlog.eu#RecipeStep"/>
        <rdfs:range rdf:resource="http://ontology.foodlog.eu#UsesIngredient"/>
        <rdfs:comment xml:lang="en">A recipe step uses an ingredient in that step</rdfs:comment>
        <rdfs:label xml:lang="en">Uses amount</rdfs:label>
    </owl:ObjectProperty>
    


    <!-- 
    ///////////////////////////////////////////////////////////////////////////////////////
    //
    // Data properties
    //
    ///////////////////////////////////////////////////////////////////////////////////////
     -->

    


    <!-- http://ontology.foodlog.eu#amount -->

    <owl:DatatypeProperty rdf:about="http://ontology.foodlog.eu#amount">
        <rdf:type rdf:resource="http://www.w3.org/2002/07/owl#FunctionalProperty"/>
        <rdfs:domain rdf:resource="http://ontology.foodlog.eu#UsesIngredient"/>
        <rdfs:range rdf:resource="http://www.w3.org/2001/XMLSchema#integer"/>
        <rdfs:comment xml:lang="en">An amount provides a measure of the quantity of ingredient used.</rdfs:comment>
        <rdfs:label xml:lang="en">amount</rdfs:label>
    </owl:DatatypeProperty>
    


    <!-- http://ontology.foodlog.eu#carbohydrates -->

    <owl:DatatypeProperty rdf:about="http://ontology.foodlog.eu#carbohydrates">
        <rdf:type rdf:resource="http://www.w3.org/2002/07/owl#FunctionalProperty"/>
        <rdfs:domain rdf:resource="http://ontology.foodlog.eu#NutritionFacts"/>
        <rdfs:range rdf:resource="http://www.w3.org/2001/XMLSchema#float"/>
        <rdfs:comment xml:lang="en">Carbohydrates denotes the amount of a nutrient present in food that is made up of a large group of organic compounds.</rdfs:comment>
        <rdfs:label xml:lang="en">carbohydrates</rdfs:label>
    </owl:DatatypeProperty>
    


    <!-- http://ontology.foodlog.eu#cuisine -->

    <owl:DatatypeProperty rdf:about="http://ontology.foodlog.eu#cuisine">
        <rdfs:domain rdf:resource="http://ontology.foodlog.eu#Recipe"/>
        <rdfs:range rdf:resource="http://www.w3.org/2001/XMLSchema#string"/>
        <rdfs:comment xml:lang="en">A style or method of cooking, especially as characteristic of a particular country, region, or establishment.</rdfs:comment>
        <rdfs:label xml:lang="en">cuisine</rdfs:label>
    </owl:DatatypeProperty>
    


    <!-- http://ontology.foodlog.eu#date -->

    <owl:DatatypeProperty rdf:about="http://ontology.foodlog.eu#date">
        <rdf:type rdf:resource="http://www.w3.org/2002/07/owl#FunctionalProperty"/>
        <rdfs:domain rdf:resource="http://ontology.foodlog.eu#Recipe"/>
        <rdfs:range rdf:resource="http://www.w3.org/2001/XMLSchema#string"/>
        <rdfs:comment xml:lang="en">A symbol containing numbers and slashes to denote the day, month and year.</rdfs:comment>
        <rdfs:label xml:lang="en">date</rdfs:label>
    </owl:DatatypeProperty>
    


    <!-- http://ontology.foodlog.eu#description -->

    <owl:DatatypeProperty rdf:about="http://ontology.foodlog.eu#description">
        <rdf:type rdf:resource="http://www.w3.org/2002/07/owl#FunctionalProperty"/>
        <rdfs:domain rdf:resource="http://ontology.foodlog.eu#Recipe"/>
        <rdfs:range rdf:resource="http://www.w3.org/2001/XMLSchema#string"/>
        <rdfs:comment xml:lang="en">A statement giving the characteristics of a recipe.</rdfs:comment>
        <rdfs:label xml:lang="en">description</rdfs:label>
    </owl:DatatypeProperty>
    


    <!-- http://ontology.foodlog.eu#energy -->

    <owl:DatatypeProperty rdf:about="http://ontology.foodlog.eu#energy">
        <rdfs:domain rdf:resource="http://ontology.foodlog.eu#NutritionFacts"/>
        <rdfs:range rdf:resource="http://www.w3.org/2001/XMLSchema#float"/>
        <rdfs:comment xml:lang="en">Energy denotes the amount of energy people get from the food and drink they consume. Commonly denoted in the unit of energy called calories.</rdfs:comment>
        <rdfs:label xml:lang="en">energy</rdfs:label>
    </owl:DatatypeProperty>
    


    <!-- http://ontology.foodlog.eu#fat -->

    <owl:DatatypeProperty rdf:about="http://ontology.foodlog.eu#fat">
        <rdfs:domain rdf:resource="http://ontology.foodlog.eu#NutritionFacts"/>
        <rdfs:range rdf:resource="http://www.w3.org/2001/XMLSchema#float"/>
        <rdfs:comment xml:lang="en">Fat denotes the amount of a nutrient present in food that is made up of natural esters of glycerol or various fatty acids.</rdfs:comment>
        <rdfs:label xml:lang="en">fat</rdfs:label>
    </owl:DatatypeProperty>
    


    <!-- http://ontology.foodlog.eu#fiber -->

    <owl:DatatypeProperty rdf:about="http://ontology.foodlog.eu#fiber">
        <rdfs:domain rdf:resource="http://ontology.foodlog.eu#NutritionFacts"/>
        <rdfs:range rdf:resource="http://www.w3.org/2001/XMLSchema#float"/>
        <rdfs:comment xml:lang="en">Fiber denotes the amount of a nutritient present in food that is made up of substances such as cellulose, lignin, and pectin, that are resistant to the action of digestive enzymes.</rdfs:comment>
        <rdfs:label xml:lang="en">fiber</rdfs:label>
    </owl:DatatypeProperty>
    


    <!-- http://ontology.foodlog.eu#ingredientName -->

    <owl:DatatypeProperty rdf:about="http://ontology.foodlog.eu#ingredientName">
        <rdf:type rdf:resource="http://www.w3.org/2002/07/owl#FunctionalProperty"/>
        <rdfs:domain rdf:resource="http://ontology.foodlog.eu#Ingredient"/>
        <rdfs:range rdf:resource="http://www.w3.org/2001/XMLSchema#string"/>
        <rdfs:comment xml:lang="en">A word or phrase that constitutes the distinctive designation of an ingredient.</rdfs:comment>
        <rdfs:label xml:lang="en">ingredient name</rdfs:label>
    </owl:DatatypeProperty>
    


    <!-- http://ontology.foodlog.eu#instruction -->

    <owl:DatatypeProperty rdf:about="http://ontology.foodlog.eu#instruction">
        <rdf:type rdf:resource="http://www.w3.org/2002/07/owl#FunctionalProperty"/>
        <rdfs:domain rdf:resource="http://ontology.foodlog.eu#RecipeStep"/>
        <rdfs:range rdf:resource="http://www.w3.org/2001/XMLSchema#string"/>
        <rdfs:comment xml:lang="en">A detailed information about how something should be done or operated.</rdfs:comment>
        <rdfs:label xml:lang="en">instruction</rdfs:label>
    </owl:DatatypeProperty>
    


    <!-- http://ontology.foodlog.eu#protein -->

    <owl:DatatypeProperty rdf:about="http://ontology.foodlog.eu#protein">
        <rdfs:domain rdf:resource="http://ontology.foodlog.eu#NutritionFacts"/>
        <rdfs:range rdf:resource="http://www.w3.org/2001/XMLSchema#float"/>
        <rdfs:comment xml:lang="en">Protein denotes the amount of a nutrient present in food that is made up of many amino acids joined together.</rdfs:comment>
        <rdfs:label xml:lang="en">protein</rdfs:label>
    </owl:DatatypeProperty>
    


    <!-- http://ontology.foodlog.eu#recipeName -->

    <owl:DatatypeProperty rdf:about="http://ontology.foodlog.eu#recipeName">
        <rdfs:domain rdf:resource="http://ontology.foodlog.eu#Recipe"/>
        <rdfs:range rdf:resource="http://www.w3.org/2001/XMLSchema#string"/>
        <rdfs:comment xml:lang="en">A word or phrase that constitutes the distinctive designation of an ingredient.</rdfs:comment>
        <rdfs:label xml:lang="en">recipe name</rdfs:label>
    </owl:DatatypeProperty>
    


    <!-- http://ontology.foodlog.eu#salt -->

    <owl:DatatypeProperty rdf:about="http://ontology.foodlog.eu#salt">
        <rdfs:domain rdf:resource="http://ontology.foodlog.eu#NutritionFacts"/>
        <rdfs:range rdf:resource="http://www.w3.org/2001/XMLSchema#float"/>
        <rdfs:comment xml:lang="en">Salt denotes the amount of a nutrient present in food that is a crystalline compound NaCl that consists of sodium chloride.</rdfs:comment>
        <rdfs:label xml:lang="en">salt</rdfs:label>
    </owl:DatatypeProperty>
    


    <!-- http://ontology.foodlog.eu#serving -->

    <owl:DatatypeProperty rdf:about="http://ontology.foodlog.eu#serving">
        <rdfs:domain rdf:resource="http://ontology.foodlog.eu#Recipe"/>
        <rdfs:range rdf:resource="http://www.w3.org/2001/XMLSchema#int"/>
        <rdfs:comment xml:lang="en">Amount of people served by the quantity of food.</rdfs:comment>
        <rdfs:label xml:lang="en">serving</rdfs:label>
    </owl:DatatypeProperty>
    


    <!-- http://ontology.foodlog.eu#stepNumber -->

    <owl:DatatypeProperty rdf:about="http://ontology.foodlog.eu#stepNumber">
        <rdfs:domain rdf:resource="http://ontology.foodlog.eu#RecipeStep"/>
        <rdfs:range rdf:resource="http://www.w3.org/2001/XMLSchema#int"/>
        <rdfs:comment xml:lang="en">Non-negative integer that is used to denote the order in a list of steps.</rdfs:comment>
        <rdfs:label xml:lang="en">step number</rdfs:label>
    </owl:DatatypeProperty>
    


    <!-- http://ontology.foodlog.eu#unit -->

    <owl:DatatypeProperty rdf:about="http://ontology.foodlog.eu#unit">
        <rdf:type rdf:resource="http://www.w3.org/2002/07/owl#FunctionalProperty"/>
        <rdfs:domain rdf:resource="http://ontology.foodlog.eu#UsesIngredient"/>
        <rdfs:range rdf:resource="http://www.w3.org/2001/XMLSchema#string"/>
        <rdfs:comment xml:lang="en">A quantity chosen as a standard in terms of which other quantities may be expressed.</rdfs:comment>
        <rdfs:label xml:lang="en">unit</rdfs:label>
    </owl:DatatypeProperty>
    


    <!-- http://ontology.foodlog.eu#variantName -->

    <owl:DatatypeProperty rdf:about="http://ontology.foodlog.eu#variantName">
        <rdfs:domain rdf:resource="http://ontology.foodlog.eu#RecipeVariant"/>
        <rdfs:range rdf:resource="http://www.w3.org/2001/XMLSchema#string"/>
        <rdfs:comment xml:lang="en">A word or phrase that constitutes the distinctive designation of a particular variant of a recipe.</rdfs:comment>
        <rdfs:label xml:lang="en">variant name</rdfs:label>
    </owl:DatatypeProperty>
    


    <!-- 
    ///////////////////////////////////////////////////////////////////////////////////////
    //
    // Classes
    //
    ///////////////////////////////////////////////////////////////////////////////////////
     -->

    


    <!-- http://ontology.foodlog.eu#AnimalOrigin -->

    <owl:Class rdf:about="http://ontology.foodlog.eu#AnimalOrigin">
        <rdfs:subClassOf rdf:resource="http://ontology.foodlog.eu#FoodType"/>
        <rdfs:comment xml:lang="en">A food type of animal origin means any food material derived from the body of an animal.</rdfs:comment>
        <rdfs:label xml:lang="en">Animal origin</rdfs:label>
    </owl:Class>
    


    <!-- http://ontology.foodlog.eu#FoodType -->

    <owl:Class rdf:about="http://ontology.foodlog.eu#FoodType">
        <rdfs:comment xml:lang="en">A food type denotes the nature or origin of an ingredient.</rdfs:comment>
        <rdfs:label xml:lang="en">Food type</rdfs:label>
    </owl:Class>
    


    <!-- http://ontology.foodlog.eu#Fruit -->

    <owl:Class rdf:about="http://ontology.foodlog.eu#Fruit">
        <rdfs:subClassOf rdf:resource="http://ontology.foodlog.eu#PlantOrigin"/>
        <owl:disjointWith rdf:resource="http://ontology.foodlog.eu#Vegetable"/>
        <rdfs:comment xml:lang="en">A food type fruit means any food material derived from fruit.</rdfs:comment>
        <rdfs:label xml:lang="en">Fruit</rdfs:label>
    </owl:Class>
    


    <!-- http://ontology.foodlog.eu#FungusOrigin -->

    <owl:Class rdf:about="http://ontology.foodlog.eu#FungusOrigin">
        <rdfs:subClassOf rdf:resource="http://ontology.foodlog.eu#FoodType"/>
        <rdfs:comment xml:lang="en">A food type of fungus origin means any food material derived from fungi like yeasts, moulds and mushrooms.</rdfs:comment>
        <rdfs:label xml:lang="en">Fungus origin</rdfs:label>
    </owl:Class>
    


    <!-- http://ontology.foodlog.eu#Ingredient -->

    <owl:Class rdf:about="http://ontology.foodlog.eu#Ingredient">
        <rdfs:comment xml:lang="en">Any of the foods or substances that are combined to make a particular dish</rdfs:comment>
        <rdfs:label xml:lang="en">Ingredient</rdfs:label>
    </owl:Class>
    


    <!-- http://ontology.foodlog.eu#NonFruitarian -->

    <owl:Class rdf:about="http://ontology.foodlog.eu#NonFruitarian">
        <rdfs:subClassOf rdf:resource="http://ontology.foodlog.eu#RecipeVariant"/>
        <rdfs:comment xml:lang="en">Recipes that are not suitable for a fruitarian diet are of the &apos;Non fruitarian&apos; class.
Meaning, recipes that contain at least one ingredient that IS NOT a fruit are &apos;Non fruitarian&apos;.</rdfs:comment>
        <rdfs:label xml:lang="en">Non fruitarian</rdfs:label>
    </owl:Class>
    


    <!-- http://ontology.foodlog.eu#NonVegan -->

    <owl:Class rdf:about="http://ontology.foodlog.eu#NonVegan">
        <rdfs:subClassOf rdf:resource="http://ontology.foodlog.eu#RecipeVariant"/>
        <rdfs:comment xml:lang="en">Recipes that are not suitable for a vegan diet are of the &apos;Non vegan&apos; class.
Meaning, recipes that contain at least one ingredient that IS of animal origin are &apos;Non vegan&apos;.</rdfs:comment>
        <rdfs:label xml:lang="en">Non vegan</rdfs:label>
    </owl:Class>
    


    <!-- http://ontology.foodlog.eu#NutritionFacts -->

    <owl:Class rdf:about="http://ontology.foodlog.eu#NutritionFacts">
        <rdfs:comment xml:lang="en">The nutrition facts of a food item describe what nutritients are in the food.</rdfs:comment>
        <rdfs:label xml:lang="en">Nutrition facts</rdfs:label>
    </owl:Class>
    


    <!-- http://ontology.foodlog.eu#PlantOrigin -->

    <owl:Class rdf:about="http://ontology.foodlog.eu#PlantOrigin">
        <rdfs:subClassOf rdf:resource="http://ontology.foodlog.eu#FoodType"/>
        <rdfs:comment xml:lang="en">A food type of plant origin means any food material derived from plants.</rdfs:comment>
        <rdfs:label xml:lang="en">Plant origin</rdfs:label>
    </owl:Class>
    


    <!-- http://ontology.foodlog.eu#Recipe -->

    <owl:Class rdf:about="http://ontology.foodlog.eu#Recipe">
        <rdfs:comment xml:lang="en">A set of instructions that describes how to prepare or make something from various ingredients.</rdfs:comment>
        <rdfs:label xml:lang="en">Recipe</rdfs:label>
    </owl:Class>
    


    <!-- http://ontology.foodlog.eu#RecipeStep -->

    <owl:Class rdf:about="http://ontology.foodlog.eu#RecipeStep">
        <rdfs:comment xml:lang="en">A stage in the process of preparing or making a recipe.</rdfs:comment>
        <rdfs:label xml:lang="en">Recipe step</rdfs:label>
    </owl:Class>
    


    <!-- http://ontology.foodlog.eu#RecipeVariant -->

    <owl:Class rdf:about="http://ontology.foodlog.eu#RecipeVariant">
        <rdfs:comment>Each recipe can have a variants and recipe variants differ slightly in the way their are prepared.</rdfs:comment>
        <rdfs:label xml:lang="en">Recipe variant</rdfs:label>
    </owl:Class>
    


    <!-- http://ontology.foodlog.eu#UsesIngredient -->

    <owl:Class rdf:about="http://ontology.foodlog.eu#UsesIngredient">
        <rdfs:comment xml:lang="en">The act of using an ingredient refers to a recipe step where a certain amount of an ingredient is used in that step.</rdfs:comment>
        <rdfs:label xml:lang="en">Uses ingredient</rdfs:label>
    </owl:Class>
    


    <!-- http://ontology.foodlog.eu#Vegetable -->

    <owl:Class rdf:about="http://ontology.foodlog.eu#Vegetable">
        <rdfs:subClassOf rdf:resource="http://ontology.foodlog.eu#PlantOrigin"/>
        <rdfs:comment xml:lang="en">A food type vegetable means any food material derived from vegetables.</rdfs:comment>
        <rdfs:label xml:lang="en">Vegetable</rdfs:label>
    </owl:Class>
    


    <!-- 
    ///////////////////////////////////////////////////////////////////////////////////////
    //
    // General axioms
    //
    ///////////////////////////////////////////////////////////////////////////////////////
     -->

    <rdf:Description>
        <rdf:type rdf:resource="http://www.w3.org/2002/07/owl#AllDisjointClasses"/>
        <owl:members rdf:parseType="Collection">
            <rdf:Description rdf:about="http://ontology.foodlog.eu#AnimalOrigin"/>
            <rdf:Description rdf:about="http://ontology.foodlog.eu#FungusOrigin"/>
            <rdf:Description rdf:about="http://ontology.foodlog.eu#PlantOrigin"/>
        </owl:members>
    </rdf:Description>
    


    <!-- 
    ///////////////////////////////////////////////////////////////////////////////////////
    //
    // Rules
    //
    ///////////////////////////////////////////////////////////////////////////////////////
     -->

    <rdf:Description rdf:about="urn:swrl:var#rv">
        <rdf:type rdf:resource="http://www.w3.org/2003/11/swrl#Variable"/>
    </rdf:Description>
    <rdf:Description rdf:about="urn:swrl:var#rs">
        <rdf:type rdf:resource="http://www.w3.org/2003/11/swrl#Variable"/>
    </rdf:Description>
    <rdf:Description rdf:about="urn:swrl:var#ui">
        <rdf:type rdf:resource="http://www.w3.org/2003/11/swrl#Variable"/>
    </rdf:Description>
    <rdf:Description rdf:about="urn:swrl:var#i">
        <rdf:type rdf:resource="http://www.w3.org/2003/11/swrl#Variable"/>
    </rdf:Description>
    <rdf:Description rdf:about="urn:swrl:var#ft">
        <rdf:type rdf:resource="http://www.w3.org/2003/11/swrl#Variable"/>
    </rdf:Description>
    <rdf:Description>
        <rdf:type rdf:resource="http://www.w3.org/2003/11/swrl#Imp"/>
        <swrl:body>
            <rdf:Description>
                <rdf:type rdf:resource="http://www.w3.org/2003/11/swrl#AtomList"/>
                <rdf:first>
                    <rdf:Description>
                        <rdf:type rdf:resource="http://www.w3.org/2003/11/swrl#ClassAtom"/>
                        <swrl:classPredicate rdf:resource="http://ontology.foodlog.eu#RecipeVariant"/>
                        <swrl:argument1 rdf:resource="urn:swrl:var#rv"/>
                    </rdf:Description>
                </rdf:first>
                <rdf:rest>
                    <rdf:Description>
                        <rdf:type rdf:resource="http://www.w3.org/2003/11/swrl#AtomList"/>
                        <rdf:first>
                            <rdf:Description>
                                <rdf:type rdf:resource="http://www.w3.org/2003/11/swrl#IndividualPropertyAtom"/>
                                <swrl:propertyPredicate rdf:resource="http://ontology.foodlog.eu#hasStep"/>
                                <swrl:argument1 rdf:resource="urn:swrl:var#rv"/>
                                <swrl:argument2 rdf:resource="urn:swrl:var#rs"/>
                            </rdf:Description>
                        </rdf:first>
                        <rdf:rest>
                            <rdf:Description>
                                <rdf:type rdf:resource="http://www.w3.org/2003/11/swrl#AtomList"/>
                                <rdf:first>
                                    <rdf:Description>
                                        <rdf:type rdf:resource="http://www.w3.org/2003/11/swrl#IndividualPropertyAtom"/>
                                        <swrl:propertyPredicate rdf:resource="http://ontology.foodlog.eu#usesAmount"/>
                                        <swrl:argument1 rdf:resource="urn:swrl:var#rs"/>
                                        <swrl:argument2 rdf:resource="urn:swrl:var#ui"/>
                                    </rdf:Description>
                                </rdf:first>
                                <rdf:rest>
                                    <rdf:Description>
                                        <rdf:type rdf:resource="http://www.w3.org/2003/11/swrl#AtomList"/>
                                        <rdf:first>
                                            <rdf:Description>
                                                <rdf:type rdf:resource="http://www.w3.org/2003/11/swrl#IndividualPropertyAtom"/>
                                                <swrl:propertyPredicate rdf:resource="http://ontology.foodlog.eu#amountOf"/>
                                                <swrl:argument1 rdf:resource="urn:swrl:var#ui"/>
                                                <swrl:argument2 rdf:resource="urn:swrl:var#i"/>
                                            </rdf:Description>
                                        </rdf:first>
                                        <rdf:rest>
                                            <rdf:Description>
                                                <rdf:type rdf:resource="http://www.w3.org/2003/11/swrl#AtomList"/>
                                                <rdf:first>
                                                    <rdf:Description>
                                                        <rdf:type rdf:resource="http://www.w3.org/2003/11/swrl#IndividualPropertyAtom"/>
                                                        <swrl:propertyPredicate rdf:resource="http://ontology.foodlog.eu#belongsTo"/>
                                                        <swrl:argument1 rdf:resource="urn:swrl:var#i"/>
                                                        <swrl:argument2 rdf:resource="urn:swrl:var#ft"/>
                                                    </rdf:Description>
                                                </rdf:first>
                                                <rdf:rest>
                                                    <rdf:Description>
                                                        <rdf:type rdf:resource="http://www.w3.org/2003/11/swrl#AtomList"/>
                                                        <rdf:first>
                                                            <rdf:Description>
                                                                <rdf:type rdf:resource="http://www.w3.org/2003/11/swrl#ClassAtom"/>
                                                                <swrl:classPredicate>
                                                                    <owl:Class>
                                                                        <owl:complementOf rdf:resource="http://ontology.foodlog.eu#Fruit"/>
                                                                    </owl:Class>
                                                                </swrl:classPredicate>
                                                                <swrl:argument1 rdf:resource="urn:swrl:var#ft"/>
                                                            </rdf:Description>
                                                        </rdf:first>
                                                        <rdf:rest rdf:resource="http://www.w3.org/1999/02/22-rdf-syntax-ns#nil"/>
                                                    </rdf:Description>
                                                </rdf:rest>
                                            </rdf:Description>
                                        </rdf:rest>
                                    </rdf:Description>
                                </rdf:rest>
                            </rdf:Description>
                        </rdf:rest>
                    </rdf:Description>
                </rdf:rest>
            </rdf:Description>
        </swrl:body>
        <swrl:head>
            <rdf:Description>
                <rdf:type rdf:resource="http://www.w3.org/2003/11/swrl#AtomList"/>
                <rdf:first>
                    <rdf:Description>
                        <rdf:type rdf:resource="http://www.w3.org/2003/11/swrl#ClassAtom"/>
                        <swrl:classPredicate rdf:resource="http://ontology.foodlog.eu#NonFruitarian"/>
                        <swrl:argument1 rdf:resource="urn:swrl:var#rv"/>
                    </rdf:Description>
                </rdf:first>
                <rdf:rest rdf:resource="http://www.w3.org/1999/02/22-rdf-syntax-ns#nil"/>
            </rdf:Description>
        </swrl:head>
    </rdf:Description>
    <rdf:Description>
        <rdf:type rdf:resource="http://www.w3.org/2003/11/swrl#Imp"/>
        <swrl:body>
            <rdf:Description>
                <rdf:type rdf:resource="http://www.w3.org/2003/11/swrl#AtomList"/>
                <rdf:first>
                    <rdf:Description>
                        <rdf:type rdf:resource="http://www.w3.org/2003/11/swrl#ClassAtom"/>
                        <swrl:classPredicate rdf:resource="http://ontology.foodlog.eu#RecipeVariant"/>
                        <swrl:argument1 rdf:resource="urn:swrl:var#rv"/>
                    </rdf:Description>
                </rdf:first>
                <rdf:rest>
                    <rdf:Description>
                        <rdf:type rdf:resource="http://www.w3.org/2003/11/swrl#AtomList"/>
                        <rdf:first>
                            <rdf:Description>
                                <rdf:type rdf:resource="http://www.w3.org/2003/11/swrl#IndividualPropertyAtom"/>
                                <swrl:propertyPredicate rdf:resource="http://ontology.foodlog.eu#hasStep"/>
                                <swrl:argument1 rdf:resource="urn:swrl:var#rv"/>
                                <swrl:argument2 rdf:resource="urn:swrl:var#rs"/>
                            </rdf:Description>
                        </rdf:first>
                        <rdf:rest>
                            <rdf:Description>
                                <rdf:type rdf:resource="http://www.w3.org/2003/11/swrl#AtomList"/>
                                <rdf:first>
                                    <rdf:Description>
                                        <rdf:type rdf:resource="http://www.w3.org/2003/11/swrl#IndividualPropertyAtom"/>
                                        <swrl:propertyPredicate rdf:resource="http://ontology.foodlog.eu#usesAmount"/>
                                        <swrl:argument1 rdf:resource="urn:swrl:var#rs"/>
                                        <swrl:argument2 rdf:resource="urn:swrl:var#ui"/>
                                    </rdf:Description>
                                </rdf:first>
                                <rdf:rest>
                                    <rdf:Description>
                                        <rdf:type rdf:resource="http://www.w3.org/2003/11/swrl#AtomList"/>
                                        <rdf:first>
                                            <rdf:Description>
                                                <rdf:type rdf:resource="http://www.w3.org/2003/11/swrl#IndividualPropertyAtom"/>
                                                <swrl:propertyPredicate rdf:resource="http://ontology.foodlog.eu#amountOf"/>
                                                <swrl:argument1 rdf:resource="urn:swrl:var#ui"/>
                                                <swrl:argument2 rdf:resource="urn:swrl:var#i"/>
                                            </rdf:Description>
                                        </rdf:first>
                                        <rdf:rest>
                                            <rdf:Description>
                                                <rdf:type rdf:resource="http://www.w3.org/2003/11/swrl#AtomList"/>
                                                <rdf:first>
                                                    <rdf:Description>
                                                        <rdf:type rdf:resource="http://www.w3.org/2003/11/swrl#IndividualPropertyAtom"/>
                                                        <swrl:propertyPredicate rdf:resource="http://ontology.foodlog.eu#belongsTo"/>
                                                        <swrl:argument1 rdf:resource="urn:swrl:var#i"/>
                                                        <swrl:argument2 rdf:resource="urn:swrl:var#ft"/>
                                                    </rdf:Description>
                                                </rdf:first>
                                                <rdf:rest>
                                                    <rdf:Description>
                                                        <rdf:type rdf:resource="http://www.w3.org/2003/11/swrl#AtomList"/>
                                                        <rdf:first>
                                                            <rdf:Description>
                                                                <rdf:type rdf:resource="http://www.w3.org/2003/11/swrl#ClassAtom"/>
                                                                <swrl:classPredicate rdf:resource="http://ontology.foodlog.eu#AnimalOrigin"/>
                                                                <swrl:argument1 rdf:resource="urn:swrl:var#ft"/>
                                                            </rdf:Description>
                                                        </rdf:first>
                                                        <rdf:rest rdf:resource="http://www.w3.org/1999/02/22-rdf-syntax-ns#nil"/>
                                                    </rdf:Description>
                                                </rdf:rest>
                                            </rdf:Description>
                                        </rdf:rest>
                                    </rdf:Description>
                                </rdf:rest>
                            </rdf:Description>
                        </rdf:rest>
                    </rdf:Description>
                </rdf:rest>
            </rdf:Description>
        </swrl:body>
        <swrl:head>
            <rdf:Description>
                <rdf:type rdf:resource="http://www.w3.org/2003/11/swrl#AtomList"/>
                <rdf:first>
                    <rdf:Description>
                        <rdf:type rdf:resource="http://www.w3.org/2003/11/swrl#ClassAtom"/>
                        <swrl:classPredicate rdf:resource="http://ontology.foodlog.eu#NonVegan"/>
                        <swrl:argument1 rdf:resource="urn:swrl:var#rv"/>
                    </rdf:Description>
                </rdf:first>
                <rdf:rest rdf:resource="http://www.w3.org/1999/02/22-rdf-syntax-ns#nil"/>
            </rdf:Description>
        </swrl:head>
    </rdf:Description>
</rdf:RDF>



<!-- Generated by the OWL API (version 4.5.9.2019-02-01T07:24:44Z) https://github.com/owlcs/owlapi -->

